SkLean/Typing2.lean
@@ -2,15 +2,61 @@ import SkLean.Ast2
 
 namespace valid_judgment
 
+lemma imp_exists_eval : valid_judgment e t → ∃ e', is_eval_once (trivial_typing e) e' := by
+  intro h_t
+  induction e
+  case m n =>
+    use SKM[(M n.succ)]
+    apply is_eval_once.m_m
+  case k n =>
+    use SKM[(K n.succ)]
+    apply is_eval_once.m_k
+  case s n =>
+    use SKM[(S n.succ)]
+    apply is_eval_once.m_s
+  case call lhs rhs ih₁ ih₂ =>
+    use SKM[(#(trivial_typing lhs) #(trivial_typing rhs))]
+    apply is_eval_once.m_call
+
+lemma call_exists_lhs_rhs_t : valid_judgment SKM[(lhs rhs)] t → ∃ t_lhs t_rhs, valid_judgment lhs t_lhs ∧ valid_judgment rhs t_rhs := by
+  intro h_t
+  cases h_t
+  case call_k x t_x t_y n h_t_x h_t_y =>
+    use (trivial_typing SKM[((K n) x)])
+    use t_y
+    exact ⟨valid_judgment.call_k₁ h_t_x, h_t_y⟩
+  case call_k₁ t_x n h_t_x =>
+    use (trivial_typing SKM[(K n)])
+    use t_x
+    exact ⟨by apply valid_judgment.k, h_t_x⟩
+  case call_s₁ t_x n h_t_x =>
+    use (trivial_typing SKM[(S n)])
+    use t_x
+    exact ⟨by apply valid_judgment.s, h_t_x⟩
+  case call_s₂ x t_x t_y n h_t_x h_t_y =>
+    use (trivial_typing SKM[((S n) x)])
+    use t_y
+    exact ⟨valid_judgment.call_s₁ h_t_x, h_t_y⟩
+  case call_s x y z t_x t_y t_call n h_t_x h_t_y h_t_z h_t_call h_u =>
+    use trivial_typing SKM[(((S n) x) y)]
+    simp_all
+    constructor
+    apply valid_judgment.call_s₂
+    exact h_t_x
+    exact h_t_y
+    use t_call
+  case call_m t n h_t =>
+    use (trivial_typing SKM[(M n)])
+    use t
+    exact ⟨valid_judgment.m n, h_t⟩
+  case call t_lhs t_rhs e' h_t_lhs h_t_rhs h_eval h_u =>
+    use t_lhs
+    use t_rhs
+
 lemma imp_m : valid_judgment e t → _root_.beta_eq (trivial_typing e) t := by
   intro h_t
   induction h_t
   repeat exact beta_eq.rfl
-  case beta_eq t₁ t₂ e' h_t₁ h_t₂ ih =>
-    apply beta_eq.symm
-    apply beta_eq.trans
-    exact (beta_eq.symm h_t₁)
-    exact (beta_eq.symm ih)
 
 theorem preservation_easy : valid_judgment e t → is_eval_once e e' → ∃ t', valid_judgment e' t' := by
   intro h_t h_eval
@@ -24,23 +70,58 @@ theorem preservation_easy : valid_judgment e t → is_eval_once e e' → ∃ t',
   case m n =>
     use trivial_typing SKM[M n]
     cases h_eval
-  case call_k x t_x n y h_t_x ih =>
+  case call_k₁ x t_x n h_t_x ih =>
+    cases h_eval
+    case left h =>
+      cases h
+  case call_s₁ x t_x n h_t_x ih =>
+    cases h_eval
+    case left h =>
+      cases h
+  case call_s₂ x t_x y t_y n h_t_x h_t_y ih₁ ih₂ =>
+    cases h_eval
+    case left h =>
+      cases h
+      case left h =>
+        cases h
+  case call_k x t_x y t_y n h_t_x h_t_y ih₁ ih₂ =>
     cases h_eval
     use t_x
-    case left lhs' a =>
-      cases a
-      case left lhs' a =>
-        cases a
-  case call_s x z y t_call n h_t_call h_u ih =>
+    case left h =>
+      cases h
+      case left h =>
+        cases h
+  case call_s x z y t_call t_x t_y t_z n h_t_call h_t_x h_t_y h_t_z h_u ih₁ ih₂ ih₃ ih₄ =>
     cases h_eval
     use t_call
-    case left lhs' a =>
-      cases a
-      case left lhs' a =>
-        cases a
-        case left lhs' a =>
-          cases a
-  case call_m e'' t' n h_t ih =>
-    
+    case left h =>
+      cases h
+      case left h =>
+        cases h
+        case left h =>
+          cases h
+  case call_m e t n h_t h_eval₂ =>
+    cases h_eval
+    case m_k n =>
+      use trivial_typing SKM[(K n.succ)]
+      apply valid_judgment.k
+    case m_s n =>
+      use trivial_typing SKM[(S n.succ)]
+      apply valid_judgment.s
+    case m_m n =>
+      use trivial_typing SKM[(M n.succ)]
+      apply valid_judgment.m
+    case m_call t' lhs rhs =>
+      use trivial_typing SKM[(#(trivial_typing lhs) #(trivial_typing rhs))]
+      have ⟨t_lhs, t_rhs, h_t_lhs, h_t_rhs⟩ := h_t.call_exists_lhs_rhs_t
+      apply valid_judgment.call
+      apply valid_judgment.call_m
+      exact h_t_lhs
+      apply valid_judgment.call_m
+      exact h_t_rhs
+      apply is_eval_once.left
+      
+      sorry
+    sorry
 
 end valid_judgment
